SIL-Parallel/Examples.thy
@@ -1,0 +1,39 @@
+theory Examples
+  imports SIL_Sound_Complete
+begin
+
+text \<open>
+  This theory contains a collection of simple example programs
+  together with proofs of their correctness using the Hoare logic
+  developed in the preceding chapters.
+\<close>
+
+subsection \<open>Skip\<close>
+
+lemma wp_normalise_example:
+  "wp (''x'' ::= ND {N 0,N 1,N 2,N 3,N 4,N 5};;
+      (IF Less (V ''x'') (N 2)
+       THEN ''x'' ::= N 2
+       ELSE SKIP);;
+      WHILE Less (V ''x'') (N 5)
+      DO ''x'' ::= Plus (V ''x'') (N 1)) (OK (\<lambda>s. s ''x'' = 5)) = (\<lambda>s. True)"
+  by force
+
+lemma normalise_example:
+  "\<turnstile> \<langle>\<lambda>s. True\<rangle>
+      ''x'' ::= ND {N 0,N 1,N 2,N 3,N 4,N 5};;
+      (IF Less (V ''x'') (N 2)
+       THEN ''x'' ::= N 2
+       ELSE SKIP);;
+      WHILE Less (V ''x'') (N 5)
+      DO ''x'' ::= Plus (V ''x'') (N 1)
+    \<langle>OK (\<lambda>s. s ''x'' = 5)\<rangle>"
+  by (smt (verit, ccfv_SIG) strengthen_pre wp_is_pre wp_normalise_example)
+
+lemma random_loop:
+  "wp (WHILE Less (V ''x'') (N 10)
+        DO ''x'' ::= ND {V ''x'',Plus (V ''x'') (N 1)}) (OK (\<lambda>s. s ''x'' = 10)) 
+    = (\<lambda>s. s ''x'' \<le> 10)"
+  oops
+
+
